theories/zoo_saturn/bqueue_mpmc__code.v
@@ -1,0 +1,223 @@
+Require Import zoo.prelude.
+Require Import zoo.language.typeclasses.
+Require Import zoo.language.notations.
+Require Import zoo_std.domain.
+Require Import zoo.options.
+
+Notation "'bqueue_mpmc٠Null'" := (
+  in_type "zoo_saturn.bqueue_mpmc.node" 0
+)(in custom zoo_tag
+).
+Notation "'bqueue_mpmc٠Node'" := (
+  in_type "zoo_saturn.bqueue_mpmc.node" 1
+)(in custom zoo_tag
+).
+
+Notation "'bqueue_mpmc٠next'" := (
+  in_type "zoo_saturn.bqueue_mpmc.node.Node" 0
+)(in custom zoo_field
+).
+Notation "'bqueue_mpmc٠data'" := (
+  in_type "zoo_saturn.bqueue_mpmc.node.Node" 1
+)(in custom zoo_field
+).
+Notation "'bqueue_mpmc٠index'" := (
+  in_type "zoo_saturn.bqueue_mpmc.node.Node" 2
+)(in custom zoo_field
+).
+Notation "'bqueue_mpmc٠estimated_capacity'" := (
+  in_type "zoo_saturn.bqueue_mpmc.node.Node" 3
+)(in custom zoo_field
+).
+
+Notation "'bqueue_mpmc٠capacity'" := (
+  in_type "zoo_saturn.bqueue_mpmc.t" 0
+)(in custom zoo_field
+).
+Notation "'bqueue_mpmc٠front'" := (
+  in_type "zoo_saturn.bqueue_mpmc.t" 1
+)(in custom zoo_field
+).
+Notation "'bqueue_mpmc٠back'" := (
+  in_type "zoo_saturn.bqueue_mpmc.t" 2
+)(in custom zoo_field
+).
+
+Definition bqueue_mpmc٠create : val :=
+  𝗳𝘂𝗻 "cap" ->
+    𝗹𝗲𝘁 "front" =
+      ‘bqueue_mpmc٠Node{ §bqueue_mpmc٠Null, (), 0, "cap" }
+    𝗶𝗻
+    { "cap", "front", "front" }.
+
+Definition bqueue_mpmc٠capacity : val :=
+  𝗳𝘂𝗻 "t" ->
+    "t".{bqueue_mpmc٠capacity}.
+
+Definition bqueue_mpmc٠size : val :=
+  𝗿𝗲𝗰 "size" "t" ->
+    𝗺𝗮𝘁𝗰𝗵 "t".{bqueue_mpmc٠front} 𝘄𝗶𝘁𝗵
+    | bqueue_mpmc٠Node ⎽ ⎽ ⎽ ⎽ 𝗮𝘀 "front" ->
+        𝗹𝗲𝘁 "front_r" = "front" 𝗶𝗻
+        𝗹𝗲𝘁 "proph" = 𝗽𝗿𝗼𝗽𝗵 𝗶𝗻
+        𝗺𝗮𝘁𝗰𝗵 "t".{bqueue_mpmc٠back} 𝘄𝗶𝘁𝗵
+        | bqueue_mpmc٠Node ⎽ ⎽ ⎽ ⎽ 𝗮𝘀 "back" ->
+            𝗹𝗲𝘁 "back_r" = "back" 𝗶𝗻
+            𝗺𝗮𝘁𝗰𝗵
+              "back_r".{bqueue_mpmc٠next}
+            𝘄𝗶𝘁𝗵
+            | bqueue_mpmc٠Node ⎽ ⎽ ⎽ ⎽ 𝗮𝘀 "node" ->
+                𝗰𝗮𝘀 "t".[bqueue_mpmc٠back] "back" "node" ⍮
+                "size" "t"
+            | bqueue_mpmc٠Null ->
+                𝗶𝗳
+                  𝗿𝗲𝘀𝗼𝗹𝘃𝗲
+                    "t".{bqueue_mpmc٠front}
+                    "proph"
+                    ()
+                  ==
+                  "front"
+                𝘁𝗵𝗲𝗻 (
+                  "back_r".{bqueue_mpmc٠index}
+                  -
+                  "front_r".{bqueue_mpmc٠index}
+                ) 𝗲𝗹𝘀𝗲 (
+                  "size" "t"
+                )
+            𝗲𝗻𝗱
+        𝗲𝗻𝗱
+    𝗲𝗻𝗱.
+
+Definition bqueue_mpmc٠is_empty : val :=
+  𝗳𝘂𝗻 "t" ->
+    𝗺𝗮𝘁𝗰𝗵 "t".{bqueue_mpmc٠front} 𝘄𝗶𝘁𝗵
+    | bqueue_mpmc٠Node ⎽ ⎽ ⎽ ⎽ 𝗮𝘀 "front_r" ->
+        "front_r".{bqueue_mpmc٠next} == §bqueue_mpmc٠Null
+    𝗲𝗻𝗱.
+
+Definition bqueue_mpmc٠fix_back : val :=
+  𝗿𝗲𝗰 "fix_back" "t" "back" "new_back" ->
+    𝗺𝗮𝘁𝗰𝗵 "new_back" 𝘄𝗶𝘁𝗵
+    | bqueue_mpmc٠Node ⎽ ⎽ ⎽ ⎽ 𝗮𝘀 "new_back_r" ->
+        𝗶𝗳
+          "new_back_r".{bqueue_mpmc٠next} == §bqueue_mpmc٠Null
+          𝗮𝗻𝗱
+          ~ 𝗰𝗮𝘀 "t".[bqueue_mpmc٠back] "back" "new_back"
+        𝘁𝗵𝗲𝗻 (
+          domain٠yield () ⍮
+          "fix_back" "t" "t".{bqueue_mpmc٠back} "new_back"
+        )
+    𝗲𝗻𝗱.
+
+#[local] Definition __zoo_recs_0 :=
+  ( 𝗿𝗲𝗰𝘀 "push_1" "t" "back" "cap" "new_back" ->
+      𝗺𝗮𝘁𝗰𝗵 "back" 𝘄𝗶𝘁𝗵
+      | bqueue_mpmc٠Node ⎽ ⎽ ⎽ ⎽ 𝗮𝘀 "back_r" ->
+          𝗺𝗮𝘁𝗰𝗵 "new_back" 𝘄𝗶𝘁𝗵
+          | bqueue_mpmc٠Node ⎽ ⎽ ⎽ ⎽ 𝗮𝘀 "new_back" ->
+              𝗹𝗲𝘁 "new_back_r" = "new_back" 𝗶𝗻
+              𝗶𝗳 "cap" == 0 𝘁𝗵𝗲𝗻 (
+                𝗺𝗮𝘁𝗰𝗵
+                  "t".{bqueue_mpmc٠front}
+                𝘄𝗶𝘁𝗵
+                | bqueue_mpmc٠Node ⎽ ⎽ ⎽ ⎽ 𝗮𝘀 "front_r" ->
+                    𝗹𝗲𝘁 "cap" =
+                      "t".{bqueue_mpmc٠capacity}
+                      -
+                      ("back_r".{bqueue_mpmc٠index}
+                       -
+                       "front_r".{bqueue_mpmc٠index})
+                    𝗶𝗻
+                    𝗶𝗳 "cap" == 0 𝘁𝗵𝗲𝗻 (
+                      false
+                    ) 𝗲𝗹𝘀𝗲 (
+                      "back_r" <-{bqueue_mpmc٠estimated_capacity} "cap" ⍮
+                      "push_1" "t" "back" "cap" "new_back"
+                    )
+                𝗲𝗻𝗱
+              ) 𝗲𝗹𝘀𝗲 (
+                "new_back_r" <-{bqueue_mpmc٠index}
+                  "back_r".{bqueue_mpmc٠index} + 1 ⍮
+                "new_back_r" <-{bqueue_mpmc٠estimated_capacity} "cap" - 1 ⍮
+                𝗶𝗳
+                  𝗰𝗮𝘀
+                    "back_r".[bqueue_mpmc٠next]
+                    §bqueue_mpmc٠Null
+                    "new_back"
+                𝘁𝗵𝗲𝗻 (
+                  bqueue_mpmc٠fix_back "t" "back" "new_back" ⍮
+                  true
+                ) 𝗲𝗹𝘀𝗲 (
+                  𝗺𝗮𝘁𝗰𝗵
+                    "back_r".{bqueue_mpmc٠next}
+                  𝘄𝗶𝘁𝗵
+                  | bqueue_mpmc٠Null ->
+                      𝗳𝗮𝗶𝗹
+                  | bqueue_mpmc٠Node ⎽ ⎽ ⎽ ⎽ 𝗮𝘀 "back" ->
+                      "push_2" "t" "back" "new_back"
+                  𝗲𝗻𝗱
+                )
+              )
+          𝗲𝗻𝗱
+      𝗲𝗻𝗱
+    𝘄𝗶𝘁𝗵 "push_2" "t" "back" "new_back" ->
+      𝗺𝗮𝘁𝗰𝗵 "back" 𝘄𝗶𝘁𝗵
+      | bqueue_mpmc٠Node ⎽ ⎽ ⎽ ⎽ 𝗮𝘀 "back" ->
+          𝗹𝗲𝘁 "back_r" = "back" 𝗶𝗻
+          "push_1"
+            "t"
+            "back"
+            "back_r".{bqueue_mpmc٠estimated_capacity}
+            "new_back"
+      𝗲𝗻𝗱
+  )%zoo_recs.
+Definition bqueue_mpmc٠push_1 :=
+  ValRecs 0 __zoo_recs_0.
+Definition bqueue_mpmc٠push_2 :=
+  ValRecs 1 __zoo_recs_0.
+#[global] Instance :
+  AsValRecs' bqueue_mpmc٠push_1 0 __zoo_recs_0 [
+    bqueue_mpmc٠push_1 ;
+    bqueue_mpmc٠push_2
+  ].
+Proof.
+  done.
+Qed.
+#[global] Instance :
+  AsValRecs' bqueue_mpmc٠push_2 1 __zoo_recs_0 [
+    bqueue_mpmc٠push_1 ;
+    bqueue_mpmc٠push_2
+  ].
+Proof.
+  done.
+Qed.
+
+Definition bqueue_mpmc٠push : val :=
+  𝗳𝘂𝗻 "t" "v" ->
+    𝗹𝗲𝘁 "new_back" =
+      ‘bqueue_mpmc٠Node{ §bqueue_mpmc٠Null, "v", 0, 0 }
+    𝗶𝗻
+    bqueue_mpmc٠push_2 "t" "t".{bqueue_mpmc٠back} "new_back".
+
+Definition bqueue_mpmc٠pop : val :=
+  𝗿𝗲𝗰 "pop" "t" ->
+    𝗺𝗮𝘁𝗰𝗵 "t".{bqueue_mpmc٠front} 𝘄𝗶𝘁𝗵
+    | bqueue_mpmc٠Node ⎽ ⎽ ⎽ ⎽ 𝗮𝘀 "front" ->
+        𝗹𝗲𝘁 "front_r" = "front" 𝗶𝗻
+        𝗺𝗮𝘁𝗰𝗵 "front_r".{bqueue_mpmc٠next} 𝘄𝗶𝘁𝗵
+        | bqueue_mpmc٠Null ->
+            §None
+        | bqueue_mpmc٠Node ⎽ ⎽ ⎽ ⎽ 𝗮𝘀 "new_front" ->
+            𝗹𝗲𝘁 "new_front_r" = "new_front" 𝗶𝗻
+            𝗶𝗳
+              𝗰𝗮𝘀 "t".[bqueue_mpmc٠front] "front" "new_front"
+            𝘁𝗵𝗲𝗻 (
+              𝗹𝗲𝘁 "v" = "new_front_r".{bqueue_mpmc٠data} 𝗶𝗻
+              "new_front_r" <-{bqueue_mpmc٠data} () ⍮
+              ‘Some( "v" )
+            ) 𝗲𝗹𝘀𝗲 (
+              domain٠yield () ⍮
+              "pop" "t"
+            )
+        𝗲𝗻𝗱
+    𝗲𝗻𝗱.
