theories/zoo_saturn/bqueue_mpmc__opaque.v
@@ -1,0 +1,11 @@
+Require Import zoo_saturn.bqueue_mpmc__code.
+
+#[global] Opaque bqueue_mpmc٠create.
+#[global] Opaque bqueue_mpmc٠capacity.
+#[global] Opaque bqueue_mpmc٠size.
+#[global] Opaque bqueue_mpmc٠is_empty.
+#[global] Opaque bqueue_mpmc٠fix_back.
+#[global] Opaque bqueue_mpmc٠push_1.
+#[global] Opaque bqueue_mpmc٠push_2.
+#[global] Opaque bqueue_mpmc٠push.
+#[global] Opaque bqueue_mpmc٠pop.
