theories/zoo_saturn/bqueue_mpmc__types.v
@@ -5,40 +5,40 @@ Require Export zoo_std.domain.
 Require Import zoo.options.
 
 Notation "'Null'" := (
-  in_type "zoo_saturn.mpmc_bqueue.node" 0
+  in_type "zoo_saturn.bqueue_mpmc.node" 0
 )(in custom zoo_tag
 ).
 Notation "'Node'" := (
-  in_type "zoo_saturn.mpmc_bqueue.node" 1
+  in_type "zoo_saturn.bqueue_mpmc.node" 1
 )(in custom zoo_tag
 ).
 
 Notation "'next'" := (
-  in_type "zoo_saturn.mpmc_bqueue.node.Node" 0
+  in_type "zoo_saturn.bqueue_mpmc.node.Node" 0
 )(in custom zoo_field
 ).
 Notation "'data'" := (
-  in_type "zoo_saturn.mpmc_bqueue.node.Node" 1
+  in_type "zoo_saturn.bqueue_mpmc.node.Node" 1
 )(in custom zoo_field
 ).
 Notation "'index'" := (
-  in_type "zoo_saturn.mpmc_bqueue.node.Node" 2
+  in_type "zoo_saturn.bqueue_mpmc.node.Node" 2
 )(in custom zoo_field
 ).
 Notation "'estimated_capacity'" := (
-  in_type "zoo_saturn.mpmc_bqueue.node.Node" 3
+  in_type "zoo_saturn.bqueue_mpmc.node.Node" 3
 )(in custom zoo_field
 ).
 
 Notation "'capacity'" := (
-  in_type "zoo_saturn.mpmc_bqueue.t" 0
+  in_type "zoo_saturn.bqueue_mpmc.t" 0
 )(in custom zoo_field
 ).
 Notation "'front'" := (
-  in_type "zoo_saturn.mpmc_bqueue.t" 1
+  in_type "zoo_saturn.bqueue_mpmc.t" 1
 )(in custom zoo_field
 ).
 Notation "'back'" := (
-  in_type "zoo_saturn.mpmc_bqueue.t" 2
+  in_type "zoo_saturn.bqueue_mpmc.t" 2
 )(in custom zoo_field
 ).
